Remove key list from abstract state.

sealing/abstract.v
@@ -1,5 +1,7 @@
-Require Import Ssreflect.ssreflect Ssreflect.ssrfun Ssreflect.ssrbool Ssreflect.eqtype Ssreflect.seq.
+Require Import Ssreflect.ssreflect Ssreflect.ssrfun Ssreflect.ssrbool.
+Require Import Ssreflect.eqtype Ssreflect.seq.
 Require Import CoqUtils.ord CoqUtils.word CoqUtils.partmap.
+Require Import CoqUtils.nominal.
 Require Import lib.utils common.types common.segment sealing.classes.
 
 Import DoNotation.
@@ -17,22 +19,10 @@ Context (mt : machine_types)
         {scr : syscall_regs mt}
         {ssa : @sealing_syscall_addrs mt}.
 
-Class sealing_key := {
-  key       : ordType;
-
-  (* This function is total, so key has to be infinite *)
-  mkkey_f : seq key -> key;
-
-  (* This ensures freshness without fixing a generation strategy *)
-  mkkey_fresh : forall ks, mkkey_f ks \notin ks
-}.
-
-Context {sk : sealing_key}.
-
 Inductive value :=
-| VData   : mword mt        -> value
-| VKey    :            key -> value
-| VSealed : mword mt -> key -> value.
+| VData   : mword mt         -> value
+| VKey    :             name -> value
+| VSealed : mword mt -> name -> value.
 
 Definition value_eq (v1 v2 : value) : bool :=
   match v1, v2 with
@@ -53,6 +43,35 @@ Qed.
 Definition value_eqMixin := EqMixin value_eqP.
 Canonical value_eqType := EqType value value_eqMixin.
 
+Definition sum_of_value v :=
+  match v with
+  | VData x => inl x
+  | VKey k => inr (inl k)
+  | VSealed x k => inr (inr (x, k))
+  end.
+
+Definition value_of_sum v :=
+  match v with
+  | inl x => VData x
+  | inr (inl k) => VKey k
+  | inr (inr (x, k)) => VSealed x k
+  end.
+
+Lemma sum_of_valueK : cancel sum_of_value value_of_sum.
+Proof. by case. Qed.
+
+Lemma value_of_sumK : cancel value_of_sum sum_of_value.
+Proof. do 3![case=>//]. Qed.
+
+Definition value_partOrdMixin := CanPartOrdMixin sum_of_valueK.
+Canonical value_partOrdType :=
+  Eval hnf in PartOrdType value value_partOrdMixin.
+Definition value_ordMixin := CanOrdMixin sum_of_valueK.
+Canonical value_ordType := Eval hnf in OrdType value value_ordMixin.
+Definition value_nominalMixin := BijNominalMixin sum_of_valueK value_of_sumK.
+Canonical value_nominalType :=
+  Eval hnf in NominalType value value_nominalMixin.
+
 Local Notation memory := {partmap mword mt -> value}.
 Local Notation registers := {partmap reg mt -> value}.
 
@@ -63,23 +82,40 @@ Local Notation "x .+1" := (x + 1) (at level 60).
 Record state := State {
   mem : memory;
   regs : registers;
-  pc : mword mt;
-  keys : seq key
+  pc : mword mt
 }.
 
 Definition state_eq (s1 s2 : state) :=
-  [&& mem s1 == mem s2, regs s1 == regs s2,
-      pc s1 == pc s2 & keys s1 == keys s2].
+  [&& mem s1 == mem s2, regs s1 == regs s2 & pc s1 == pc s2].
 
 Lemma state_eqP : Equality.axiom state_eq.
 Proof.
 move=> s1 s2; apply/(iffP idP) => [|<- {s2}].
-  by case: s1 s2=> [????] [????] /and4P [/= /eqP -> /eqP -> /eqP -> /eqP ->].
-by case: s1 => [????]; rewrite /state_eq !eqxx.
+  by case: s1 s2=> [???] [???] /and3P [/= /eqP -> /eqP -> /eqP ->].
+by case: s1 => [???]; rewrite /state_eq !eqxx.
 Qed.
 
 Definition state_eqMixin := EqMixin state_eqP.
 Canonical state_eqType := EqType state state_eqMixin.
+
+Definition tuple_of_state (s : state) := (mem s, regs s, pc s).
+Definition state_of_tuple s := let: (m, rs, pc) := s in State m rs pc.
+
+Lemma tuple_of_stateK : cancel tuple_of_state state_of_tuple.
+Proof. by case. Qed.
+
+Lemma state_of_tupleK : cancel state_of_tuple tuple_of_state.
+Proof. by do 2!case. Qed.
+
+Definition state_partOrdMixin := CanPartOrdMixin tuple_of_stateK.
+Canonical state_partOrdType :=
+  Eval hnf in PartOrdType state state_partOrdMixin.
+Definition state_ordMixin := CanOrdMixin tuple_of_stateK.
+Canonical state_ordType := Eval hnf in OrdType state state_ordMixin.
+Definition state_nominalMixin :=
+  BijNominalMixin tuple_of_stateK state_of_tupleK.
+Canonical state_nominalType :=
+  Eval hnf in NominalType state state_nominalMixin.
 
 Definition syscall_addrs := [:: mkkey_addr; seal_addr; unseal_addr].
 
@@ -92,145 +128,144 @@ Definition decode (mem : memory) (pc : mword mt) :=
   end.
 
 Inductive step (st st' : state) : Prop :=
-| step_nop : forall mem reg pc ks
-    (ST   : st = State mem reg pc ks)
+| step_nop : forall mem reg pc
+    (ST   : st = State mem reg pc)
     (INST : decode mem pc =? Nop _)
-    (NEXT : st' = State mem reg (pc.+1) ks),   step st st'
-| step_const : forall mem reg reg' pc n r ks
-    (ST   : st = State mem reg pc ks)
+    (NEXT : st' = State mem reg (pc.+1)),   step st st'
+| step_const : forall mem reg reg' pc n r
+    (ST   : st = State mem reg pc)
     (INST : decode mem pc =? Const n r)
     (UPD  : updm reg r (VData (swcast n)) =? reg')
-    (NEXT : st' = State mem reg' (pc.+1) ks),   step st st'
-| step_mov : forall mem reg reg' pc r1 v1 r2 ks
-    (ST   : st = State mem reg pc ks)
+    (NEXT : st' = State mem reg' (pc.+1)),   step st st'
+| step_mov : forall mem reg reg' pc r1 v1 r2
+    (ST   : st = State mem reg pc)
     (INST : decode mem pc =? Mov r1 r2)
     (R1W  : reg r1 =? v1)
     (UPD  : updm reg r2 v1 =? reg')
-    (NEXT : st' = State mem reg' (pc.+1) ks),   step st st'
-| step_binop : forall mem reg reg' pc op r1 r2 r3 w1 w2 ks
-    (ST   : st = State mem reg pc ks)
+    (NEXT : st' = State mem reg' (pc.+1)),   step st st'
+| step_binop : forall mem reg reg' pc op r1 r2 r3 w1 w2
+    (ST   : st = State mem reg pc)
     (INST : decode mem pc =? Binop op r1 r2 r3)
     (R1W  : reg r1 =? VData w1)
     (R2W  : reg r2 =? VData w2)
     (UPD  : updm reg r3 (VData (binop_denote op w1 w2)) =? reg')
-    (NEXT : st' = State mem reg' (pc.+1) ks),   step st st'
-| step_load : forall mem reg reg' pc r1 r2 w1 v2 ks
-    (ST   : st = State mem reg pc ks)
+    (NEXT : st' = State mem reg' (pc.+1)),   step st st'
+| step_load : forall mem reg reg' pc r1 r2 w1 v2
+    (ST   : st = State mem reg pc)
     (INST : decode mem pc =? Load r1 r2)
     (R1W  : reg r1 =? VData w1)
     (MEM1 : mem w1 =? v2)
     (UPD  : updm reg r2 v2 =? reg')
-    (NEXT : st' = State mem reg' (pc.+1) ks),   step st st'
-| step_store : forall mem mem' reg pc r1 r2 w1 v2 ks
-    (ST   : st = State mem reg pc ks)
+    (NEXT : st' = State mem reg' (pc.+1)),   step st st'
+| step_store : forall mem mem' reg pc r1 r2 w1 v2
+    (ST   : st = State mem reg pc)
     (INST : decode mem pc =? Store r1 r2)
     (R1W  : reg r1 =? VData w1)
     (R2W  : reg r2 =? v2)
     (UPDM : updm mem w1 v2 =? mem')
-    (NEXT : st' = State mem' reg (pc.+1) ks),   step st st'
-| step_jump : forall mem reg pc r w ks
-    (ST   : st = State mem reg pc ks)
+    (NEXT : st' = State mem' reg (pc.+1)),   step st st'
+| step_jump : forall mem reg pc r w
+    (ST   : st = State mem reg pc)
     (INST : decode mem pc =? Jump r)
     (RW   : reg r =? VData w)
-    (NEXT : st' = State mem reg w ks),   step st st'
-| step_bnz : forall mem reg pc r n w ks
-    (ST   : st = State mem reg pc ks)
+    (NEXT : st' = State mem reg w),   step st st'
+| step_bnz : forall mem reg pc r n w
+    (ST   : st = State mem reg pc)
     (INST : decode mem pc =? Bnz r n)
     (RW   : reg r =? VData w),
     let pc' := pc + (if w == 0
                      then 1 else swcast n) in forall
-    (NEXT : st' = State mem reg pc' ks),   step st st'
-| step_jal : forall mem reg reg' pc r w ks
-    (ST   : st = State mem reg pc ks)
+    (NEXT : st' = State mem reg pc'),   step st st'
+| step_jal : forall mem reg reg' pc r w
+    (ST   : st = State mem reg pc)
     (INST : decode mem pc =? Jal r)
     (RW   : reg r =? VData w)
     (UPD  : updm reg ra (VData (pc.+1)) =? reg')
-    (NEXT : st' = State mem reg' w ks),   step st st'
-| step_mkkey : forall mem reg reg' pc ks
-    (ST   : st = State mem reg mkkey_addr ks)
+    (NEXT : st' = State mem reg' w),   step st st'
+| step_mkkey : forall mem reg reg' pc
+    (ST   : st = State mem reg mkkey_addr)
     (INST : decode mem mkkey_addr = None)
-    (UPD  : updm reg syscall_ret (VKey (mkkey_f ks)) =? reg')
+    (UPD  : updm reg syscall_ret (VKey (fresh (names st))) =? reg')
     (RET  : reg ra =? VData pc)
-    (NEXT : st' = State mem reg' pc ((mkkey_f ks) :: ks)),   step st st'
-| step_seal : forall mem reg reg' pc ks payload key
-    (ST   : st = State mem reg seal_addr ks)
+    (NEXT : st' = State mem reg' pc),   step st st'
+| step_seal : forall mem reg reg' pc payload key
+    (ST   : st = State mem reg seal_addr)
     (INST : decode mem seal_addr = None)
     (R1   : reg syscall_arg1 =? VData payload)
     (R2   : reg syscall_arg2 =? VKey key)
     (UPD  : updm reg syscall_ret (VSealed payload key) =? reg')
     (RET  : reg ra =? VData pc)
-    (NEXT : st' = State mem reg' pc ks),   step st st'
-| step_unseal : forall mem reg reg' pc ks payload key
-    (ST   : st = State mem reg unseal_addr ks)
+    (NEXT : st' = State mem reg' pc),   step st st'
+| step_unseal : forall mem reg reg' pc payload key
+    (ST   : st = State mem reg unseal_addr)
     (INST : decode mem unseal_addr = None)
     (R1   : reg syscall_arg1 =? VSealed payload key)
     (R2   : reg syscall_arg2 =? VKey key)
     (UPD  : updm reg syscall_ret (VData payload) =? reg')
     (RET  : reg ra =? VData pc)
-    (NEXT : st' = State mem reg' pc ks),   step st st'.
+    (NEXT : st' = State mem reg' pc),   step st st'.
 
 Definition stepf (st : state) : option state :=
-  let 'State mem reg pc keys := st in
+  let 'State mem reg pc := st in
   match decode mem pc with
     | Some Nop =>
-      Some (State mem reg (pc.+1) keys)
+      Some (State mem reg (pc.+1))
     | Some (Const n r) =>
       do! reg' <- updm reg r (VData (swcast n));
-      Some (State mem reg' (pc.+1) keys)
+      Some (State mem reg' (pc.+1))
     | Some (Mov r1 r2) =>
       do! v <- reg r1;
       do! reg' <- updm reg r2 v;
-      Some (State mem reg' (pc.+1) keys)
+      Some (State mem reg' (pc.+1))
     | Some (Binop b r1 r2 r3) =>
       do! v1 <- reg r1;
       do! v2 <- reg r2;
       if v1 is VData i1 then if v2 is VData i2 then
         do! reg' <- updm reg r3 (VData (binop_denote b i1 i2));
-        Some (State mem reg' (pc.+1) keys)
+        Some (State mem reg' (pc.+1))
       else None else None
     | Some (Load r1 r2) =>
       do! v <- reg r1;
       if v is VData i then
         do! v' <- mem i;
         do! reg' <- updm reg r2 v';
-        Some (State mem reg' (pc.+1) keys)
+        Some (State mem reg' (pc.+1))
       else None
     | Some (Store r1 r2) =>
       do! v1 <- reg r1;
       do! v2 <- reg r2;
       if v1 is VData i1 then
         do! mem' <- updm mem i1 v2;
-        Some (State mem' reg (pc.+1) keys)
+        Some (State mem' reg (pc.+1))
       else None
     | Some (Jump r) =>
       do! v <- reg r;
       if v is VData i then
-        Some (State mem reg i keys)
+        Some (State mem reg i)
       else None
     | Some (Bnz r n) =>
       do! vr <- reg r;
       if vr is VData c then
         let pc' := pc + if c == 0
                         then 1 else swcast n in
-        Some (State mem reg pc' keys)
+        Some (State mem reg pc')
       else None
     | Some (Jal r) =>
       do! vr <- reg r;
       if vr is VData i then
         do! reg' <- updm reg ra (VData (pc.+1));
-        Some (State mem reg' i keys)
+        Some (State mem reg' i)
       else None
     | Some JumpEpc | Some AddRule | Some (GetTag _ _)
     | Some (PutTag _ _ _) | Some Halt =>
     None
     | None =>
     if pc == mkkey_addr then
-      let k := mkkey_f keys in
-      let keys' := k :: keys in
+      let k := fresh (names st) in
       do! reg' <- updm reg syscall_ret (VKey k);
       do! ret <- reg ra;
       if ret is VData pc' then
-        Some (State mem reg' pc' keys')
+        Some (State mem reg' pc')
       else None
     else if pc == seal_addr then
       do! v1 <- reg syscall_arg1;
@@ -239,7 +274,7 @@ Definition stepf (st : state) : option state :=
         do! reg' <- updm reg syscall_ret (VSealed payload k);
         do! ret <- reg ra;
         if ret is VData pc' then
-          Some (State mem reg' pc' keys)
+          Some (State mem reg' pc')
         else None
       else None else None
     else if pc == unseal_addr then
@@ -250,7 +285,7 @@ Definition stepf (st : state) : option state :=
           do! reg' <- updm reg syscall_ret (VData payload);
           do! ret <- reg ra;
           if ret is VData pc' then
-            Some (State mem reg' pc' keys)
+            Some (State mem reg' pc')
           else None
         else None
       else None else None
@@ -285,18 +320,19 @@ Program Definition abstract_initial_state
   {|
     mem := mem;
     regs := regs;
-    pc := base_addr;
-    keys := [::]
+    pc := base_addr
   |}.
 
 End WithClasses.
 
-Notation memory mt := {partmap mword mt -> @value mt _}.
-Notation registers mt := {partmap reg mt -> @value mt _}.
+Notation memory mt := {partmap mword mt -> @value mt}.
+Notation registers mt := {partmap reg mt -> @value mt}.
 
 End Abs.
 
-Arguments Abs.state mt {_}.
+Arguments Abs.state mt.
 
 Canonical Abs.value_eqType.
+Canonical Abs.value_nominalType.
 Canonical Abs.state_eqType.
+Canonical Abs.state_nominalType.
